# Combining Like Terms

## What are Like Terms?

Like terms are terms that have the exact same variable part (same letter and same exponent). Only the numbers in front (coefficients) can be different. You can combine like terms by adding or subtracting their coefficients.

**Key idea:** You can only combine things that are alike!

Like terms:
- 3x and 5x (both have x)
- 2y² and -7y² (both have y²)
- 4 and 9 (both are constants)

NOT like terms:
- 3x and 3y (different variables)
- 2x and 2x² (different exponents)
- 5a and 5b (different variables)

## How to Solve

Follow these steps to combine like terms:

1. **Identify like terms** - Group terms with same variable parts
2. **Add or subtract coefficients** - Combine the numbers in front
3. **Keep the variable part** - The variable stays the same
4. **Arrange terms** - Usually put in order (x², x, constants)
5. **Check** - Make sure no more like terms can be combined

## Step-by-Step Example

**Simplify:** 3x + 5 + 2x - 1

### Step 1: Identify like terms
```
x-terms: 3x and 2x
Constants: 5 and -1
```

### Step 2: Combine x-terms
Add the coefficients:
```
3x + 2x = (3 + 2)x = 5x
```

### Step 3: Combine constants
```
5 + (-1) = 5 - 1 = 4
```

### Step 4: Write final answer
```
3x + 5 + 2x - 1 = 5x + 4
```

### Step 5: Check your answer
Substitute x = 2:
```
Original: 3(2) + 5 + 2(2) - 1 = 6 + 5 + 4 - 1 = 14
Simplified: 5(2) + 4 = 10 + 4 = 14 ✓
```

## More Examples

### Example 2: Multiple variables
**Simplify:** 4x + 3y - 2x + 5y

```
x-terms: 4x - 2x = 2x
y-terms: 3y + 5y = 8y

Answer: 2x + 8y
```

**Check:** Let x = 1, y = 2
```
Original: 4(1) + 3(2) - 2(1) + 5(2) = 4 + 6 - 2 + 10 = 18
Simplified: 2(1) + 8(2) = 2 + 16 = 18 ✓
```

### Example 3: Different exponents
**Simplify:** 2x² + 5x - x² + 3x - 7

```
x²-terms: 2x² - x² = 1x² = x²
x-terms: 5x + 3x = 8x
Constants: -7

Answer: x² + 8x - 7
```

**Check:** Let x = 2
```
Original: 2(4) + 5(2) - (4) + 3(2) - 7 = 8 + 10 - 4 + 6 - 7 = 13
Simplified: (4) + 8(2) - 7 = 4 + 16 - 7 = 13 ✓
```

### Example 4: Negative coefficients
**Simplify:** -3a + 8 - 5a - 2

```
a-terms: -3a - 5a = -8a
Constants: 8 - 2 = 6

Answer: -8a + 6
```

**Check:** Let a = 1
```
Original: -3(1) + 8 - 5(1) - 2 = -3 + 8 - 5 - 2 = -2
Simplified: -8(1) + 6 = -8 + 6 = -2 ✓
```

## Key Points to Remember

✓ **Same variable AND exponent** - Both must match to combine
✓ **Add/subtract coefficients only** - The variable part stays the same
✓ **Constants combine too** - Plain numbers are like terms with each other
✓ **Watch signs** - Be careful with negative coefficients
✓ **Cannot combine different variables** - 3x and 4y stay separate
✓ **Coefficient of 1** - Remember x = 1x

## Common Mistakes to Avoid

❌ **Combining unlike terms** - Wrong: 3x + 4y = 7xy
✓ Correct: 3x + 4y cannot be combined

❌ **Changing the variable** - Wrong: 2x + 3x = 5x²
✓ Correct: 2x + 3x = 5x

❌ **Multiplying instead of adding** - Wrong: 3x + 2x = 6x²
✓ Correct: 3x + 2x = 5x

❌ **Ignoring signs** - Wrong: 5x - 3x = 8x
✓ Correct: 5x - 3x = 2x

## Practice More

[Khan Academy: Combining Like Terms](https://www.khanacademy.org/math/algebra-basics/alg-basics-algebraic-expressions/alg-basics-combining-like-terms/v/combining-like-terms)

---

**Next Skills:**
- Distributive Property
- Solving Multi-Step Equations
- Factoring Expressions
